Setlec/SetR/Interp2/EnvS2U.lean
@@ -1,5 +1,5 @@
 import Setlec.SetR.Annot.EnvS2U
-import Setlec.SetR.Interp2.Install2
+import Setlec.SetBase.Install2
 import Setlec.SetR.Interp2.Step2.Whnf
 
 /-!
